<?xml version="1.0" encoding="UTF-8"?>
<rdf:RDF
   xmlns:cc="http://creativecommons.org/ns#"
   xmlns:dc="http://purl.org/dc/elements/1.1/"
   xmlns:owl="http://www.w3.org/2002/07/owl#"
   xmlns:rdf="http://www.w3.org/1999/02/22-rdf-syntax-ns#"
   xmlns:rdfs="http://www.w3.org/2000/01/rdf-schema#"
   xmlns:skos="http://www.w3.org/2004/02/skos/core#"
>
  <rdf:Description rdf:about="http://purl.org/asc/1297.0/1993/toa/0.2">
    <rdf:type rdf:resource="http://www.w3.org/2004/02/skos/core#ConceptScheme"/>
    <rdf:type rdf:resource="http://www.w3.org/2002/07/owl#Ontology"/>
    <owl:versionInfo rdf:resource="http://purl.org/asc/1297.0/1993/toa/0.2"/>
    <cc:morePermissions rdf:resource="http://www.abs.gov.au/ausstats/abs@.nsf/mf/1297.0"/>
    <rdfs:label>TOA 1993 Ontology</rdfs:label>
    <dc:creator>University of Southern Queensland</dc:creator>
    <dc:creator>Griffith University</dc:creator>
    <cc:license rdf:resource="http://creativecommons.org/licenses/by-nc/3.0/au/"/>
    <owl:priorVersion rdf:resource="http://purl.org/asc/1297.0/1993/toa/0.1"/>
    <dc:title xml:lang="en">Australian and New Zealand Standard Research Classification (ANZSRC): Type of Activity.</dc:title>
    <dc:source rdf:resource="http://www.abs.gov.au/AUSSTATS/abs@.nsf/allprimarymainfeatures/5D99AEA1DD8AA8E0CA2574180005421C"/>
    <dc:rights>The source data is published by the Australian Bureau of Statistics, and can be found at the following address: http://www.abs.gov.au/ausstats/abs@.nsf/0/4AE1B46AE2048A28CA25741800044242 . This document is published under the Creative Commons Attribution License 3.0 Australia.</dc:rights>
    <rdfs:seeAlso rdf:resource="http://www.abs.gov.au/ausstats/abs@.nsf/mf/1297.0"/>
    <rdfs:comment>An ontology that provides classes codes and hierarchical information about ASRC/ANZSRC Type of Activity definitions.</rdfs:comment>
    <dc:date>2012-04-05</dc:date>
  </rdf:Description>
  <rdf:Description rdf:about="http://purl.org/asc/1297.0/1993/toa/">
    <skos:hasTopConcept rdf:resource="http://purl.org/asc/1297.0/1993/toa/PureBasicResearch"/>
    <skos:hasTopConcept rdf:resource="http://purl.org/asc/1297.0/1993/toa/ExperimentalDevelopment"/>
    <skos:hasTopConcept rdf:resource="http://purl.org/asc/1297.0/1993/toa/StrategicBasicResearch"/>
    <skos:hasTopConcept rdf:resource="http://purl.org/asc/1297.0/1993/toa/AppliedResearch"/>
    <rdf:type rdf:resource="http://www.w3.org/2004/02/skos/core#ConceptScheme"/>
    <rdf:type rdf:resource="http://www.w3.org/2002/07/owl#Ontology"/>
    <owl:versionInfo rdf:resource="http://purl.org/asc/1297.0/1993/toa/0.2"/>
    <cc:morePermissions rdf:resource="http://www.abs.gov.au/ausstats/abs@.nsf/mf/1297.0"/>
    <rdfs:label>TOA 1993 Ontology</rdfs:label>
    <dc:creator>University of Southern Queensland</dc:creator>
    <dc:creator>Griffith University</dc:creator>
    <cc:license rdf:resource="http://creativecommons.org/licenses/by-nc/3.0/au/"/>
    <owl:priorVersion rdf:resource="http://purl.org/asc/1297.0/1993/toa/0.1"/>
    <dc:title xml:lang="en">Australian and New Zealand Standard Research Classification (ANZSRC): Type of Activity.</dc:title>
    <dc:source rdf:resource="http://www.abs.gov.au/AUSSTATS/abs@.nsf/allprimarymainfeatures/5D99AEA1DD8AA8E0CA2574180005421C"/>
    <dc:rights>The source data is published by the Australian Bureau of Statistics, and can be found at the following address: http://www.abs.gov.au/ausstats/abs@.nsf/0/4AE1B46AE2048A28CA25741800044242 . This document is published under the Creative Commons Attribution License 3.0 Australia.</dc:rights>
    <rdfs:seeAlso rdf:resource="http://www.abs.gov.au/ausstats/abs@.nsf/mf/1297.0"/>
    <rdfs:comment>An ontology that provides classes codes and hierarchical information about ASRC/ANZSRC Type of Activity definitions.</rdfs:comment>
    <dc:date>2012-04-05</dc:date>
  </rdf:Description>
  <rdf:Description rdf:about="http://purl.org/asc/1297.0/1993/toa/TOA">
    <rdfs:label>TOA 1993 Definition</rdfs:label>
    <rdf:type rdf:resource="http://www.w3.org/2002/07/owl#Class"/>
    <rdfs:comment>Instances of this class describe TOA definitions</rdfs:comment>
    <rdfs:subClassOf rdf:resource="http://www.w3.org/2004/02/skos/core#Concept"/>
  </rdf:Description>
  <rdf:Description rdf:about="http://purl.org/asc/1297.0/1993/toa/PureBasicResearch">
    <rdfs:label>Pure basic research</rdfs:label>
    <rdf:type rdf:resource="http://www.w3.org/2002/07/owl#Thing"/>
    <rdf:type rdf:resource="http://purl.org/asc/1297.0/1993/toa/TOA"/>
    <rdfs:comment>Pure basic research is experimental and theoretical work undertaken to acquire new knowledge without looking for long term benefits other than the advancement of knowledge.</rdfs:comment>
    <skos:inScheme rdf:resource="http://purl.org/asc/1297.0/1993/toa/"/>
    <skos:prefLabel xml:lang="en">Pure basic research</skos:prefLabel>
  </rdf:Description>
  <rdf:Description rdf:about="http://purl.org/asc/1297.0/1993/toa/ExperimentalDevelopment">
    <rdfs:label>Experimental development</rdfs:label>
    <rdf:type rdf:resource="http://www.w3.org/2002/07/owl#Thing"/>
    <rdf:type rdf:resource="http://purl.org/asc/1297.0/1993/toa/TOA"/>
    <rdfs:comment>Experimental development is systematic work, using existing knowledge gained from research or practical experience, that is directed to producing new materials, products or devices, to installing new processes, systems and services, or to improving substantially those already produced or installed.</rdfs:comment>
    <skos:inScheme rdf:resource="http://purl.org/asc/1297.0/1993/toa/"/>
    <skos:prefLabel xml:lang="en">Experimental development</skos:prefLabel>
  </rdf:Description>
  <rdf:Description rdf:about="http://purl.org/asc/1297.0/1993/toa/AppliedResearch">
    <rdfs:label>Applied research</rdfs:label>
    <rdf:type rdf:resource="http://www.w3.org/2002/07/owl#Thing"/>
    <rdf:type rdf:resource="http://purl.org/asc/1297.0/1993/toa/TOA"/>
    <rdfs:comment>Applied research is original work undertaken primarily to acquire new knowledge with a specific application in view. It is undertaken either to determine possible uses for the findings of basic research or to determine new ways of achieving some specific and predetermined objectives.</rdfs:comment>
    <skos:inScheme rdf:resource="http://purl.org/asc/1297.0/1993/toa/"/>
    <skos:prefLabel xml:lang="en">Applied research</skos:prefLabel>
  </rdf:Description>
  <rdf:Description rdf:about="http://purl.org/asc/1297.0/1993/toa/StrategicBasicResearch">
    <rdfs:label>Strategic basic research</rdfs:label>
    <rdf:type rdf:resource="http://www.w3.org/2002/07/owl#Thing"/>
    <rdf:type rdf:resource="http://purl.org/asc/1297.0/1993/toa/TOA"/>
    <rdfs:comment>Strategic basic research is experimental and theoretical work undertaken to acquire new knowledge directed into specified broad areas in the expectation of useful discoveries. It provides the broad base of knowledge necessary for the solution of recognised practical problems.</rdfs:comment>
    <skos:inScheme rdf:resource="http://purl.org/asc/1297.0/1993/toa/"/>
    <skos:prefLabel xml:lang="en">Strategic basic research</skos:prefLabel>
  </rdf:Description>
</rdf:RDF>
